

Home work

0-1-0 = one-to-one

Sec 1

32

a) add is not 0-1-0 since, for example,
 $\text{add}(1, 1) = \text{add}(0, 2)$ while $(1, 1) \neq (0, 2)$.

It is onto, however

$y \in \mathbb{R}$ $y = \text{add}(x)$ solution $x = (y, 0)$

b) is not 0-1-0

$$\text{mult}(1, 4) = \text{mult}(2, 2)$$

while

$$(1, 4) \neq (2, 2)$$

$y \in \mathbb{R}$ $y = \text{mult}(x)$ $x = (y, 1)$

all

~~a) with is not 0-1-0~~

32

a) h isn't 0-1-0: $h(3) = 3 = h(-1)$ $3 \neq -1$

b) h is 0-1-0: $h(x_1) = h(x_2)$

$$x_1^2 + 2 = x_2^2 + 2$$

$$x_1^2 = x_2^2 \quad x_1 = \pm x_2$$

88

a)

$$f(x) = (x+2)^2 - 100$$

$$f(x_1) = f(x_2)$$

$$(x_1+2)^2 - 100 = (x_2+2)^2 - 100$$

$$(x_1+2)^2 = (x_2+2)^2$$

$$|x_1+2| = |x_2+2|$$

$$x_1, x_2 \in \mathbb{N}$$

$$x_1+2 > 0$$

$$x_2+2 > 0$$

$$x_1+2 = x_2+2$$

$$x_1 = x_2$$

$$\text{if } 0+2=0$$

b) is not 0+2=0

$$f(0) = f(-14) = (-51)$$

it is not onto

c) It is not 0+2=0

$$f(0) = f(-14)$$

$$y = -100$$

Sec 2

1. Let $y = f(x)$

$$x = f(y) = -\sqrt{y-1}$$

$$y = x^2 = f^{-1}(x)$$

So.

a) $f \circ g = \{(3,1), (3,8), (2,3), (9,9), (5,3)\}$

g o f is not $f = \{1, 2, 3, 8, 9\} \notin \text{dom}$

$$g = \{1, 2, 3, 4, 5\}$$

f o f is not $f = \{1, 2, 3, 8, 9\} \notin \text{dom}$

$$f = \{1, 2, 3, 4, 5\}$$

$$g \circ g = \{(1,2), (2,3), (3,2), (4,3), (5,2)\}$$

c) Since f is not 0 and onto, it has an inverse $f^{-1} = \{(8,3), (9,3), (3,4), (1,2), (2,3)\}$
 & y is not 0+2=0 of g is not onto

$$\int_0^3 f(x) = \frac{1}{x} \Big|_0^3 = \frac{1}{3} - \frac{1}{0} = -\frac{1}{3}$$

$$\int_0^2 f(x) = \frac{x+1}{x} \Big|_0^2 = \frac{2+1}{2} - \frac{0+1}{0} = \frac{3}{2} - \frac{1}{0} = -\frac{1}{2}$$

$$\int_0^2 f(x) = \frac{x}{x+1} \Big|_0^2 = \frac{2}{2+1} - \frac{0}{0+1} = \frac{2}{3} - 0 = \frac{2}{3}$$

$$\int_0^2 f(x) = \frac{1}{x+1} \Big|_0^2 = \frac{1}{2+1} - \frac{1}{0+1} = \frac{1}{3} - 1 = -\frac{2}{3}$$

5 (a)

$$g(m, n_1) = g(m_2, n_2)$$

$$(m_1, f(n_1)) = (m_2, f(n_2))$$

$$m_1 = m_2$$

$$f(n_1) = f(n_2)$$

f is one-to-one $n_1 = n_2$

g is one-to-one

$$(m, n_1) = (m_2, n_2)$$

g is onto let $(a, b) \in \mathbb{N} \times \mathbb{Z}$

f is onto $n \in \mathbb{N}$

$$f(n) = b$$

$$g(a, n) = (a, f(n)) = (a, b)$$

g is onto

b) Let $f: N \rightarrow Z$ be any $0 \neq 1 \neq 0$ onto function (for example, the sign of subtraction operator)

$$g: N \times N \rightarrow N \times Z$$

$$g(m, h) = (m, f(h))$$

$$\text{is } 0 \neq 1 \neq 0$$

$$N \times N \rightarrow N \times Z$$

$$12 \text{ a) } f(x) = kx + c$$

$$f(1) = 1 + 1$$

$$b) f(x) = 2x + 4$$

$$\text{is } 0 \neq 1 \neq 0$$

$$(c, d) \text{ and } (e, f)$$

c)

$$f: (0, 1) \rightarrow (0, 1)$$

$$f(x) = a + (b-a)x \text{ is } 0 \neq 1 \neq 0$$

$$g: (0, 1) \rightarrow (c, d)$$

$$g(x) = c + (d-c)x$$

$$f^{-1} \text{ provides } 0 \neq 1 \neq 0$$

$$(b, d) \rightarrow (c, d)$$

$$g \circ f^{-1}(x) = c + \frac{d-c}{b-a}(x-a)$$